fixed

Primitive_Matchers/IPSpace_Matcher.thy
@@ -7,11 +7,12 @@ begin
 
 subsection{*Primitive Matchers: IP Space Matcher*}
 
-(*TODO refactor: use ipv4s_to_set*)
+(*for the first 4 cases, we set up better simp rules. this formulation is required such that simple_matcher is executable*)
 fun simple_matcher :: "(iptrule_match, packet) exact_match_tac" where
-  "simple_matcher (Src ip) p = bool_to_ternary (src_ip p \<in> ipv4s_to_set ip)" |
-
-  "simple_matcher (Dst ip) p = bool_to_ternary (dst_ip p \<in> ipv4s_to_set ip)" |
+  "simple_matcher (Src (Ip4Addr ip)) p = bool_to_ternary (ipv4addr_of_dotteddecimal ip = src_ip p)" |
+  "simple_matcher (Src (Ip4AddrNetmask ip n)) p = bool_to_ternary (src_ip p \<in> ipv4range_set_from_bitmask (ipv4addr_of_dotteddecimal ip) n)" |
+  "simple_matcher (Dst (Ip4Addr ip)) p = bool_to_ternary (ipv4addr_of_dotteddecimal ip = dst_ip p)" |
+  "simple_matcher (Dst (Ip4AddrNetmask ip n)) p = bool_to_ternary (dst_ip p \<in> ipv4range_set_from_bitmask (ipv4addr_of_dotteddecimal ip) n)" |
 
   "simple_matcher (Prot ProtAll) _ = TernaryTrue" |
   "simple_matcher (Prot ipt_protocol.ProtTCP) p = bool_to_ternary (prot p = protPacket.ProtTCP)" |
@@ -20,16 +21,19 @@ fun simple_matcher :: "(iptrule_match, packet) exact_match_tac" where
   "simple_matcher (Extra _) p = TernaryUnknown"
 
 
-declare simple_matcher.simps(1)[code del]
-declare simple_matcher.simps(2)[code del]
-lemma [code_unfold]:
-  "simple_matcher (Src (Ip4Addr ip)) p = bool_to_ternary (ipv4addr_of_dotteddecimal ip = src_ip p)" 
-  "simple_matcher (Src (Ip4AddrNetmask ip n)) p = bool_to_ternary (src_ip p \<in> ipv4range_set_from_bitmask (ipv4addr_of_dotteddecimal ip) n)"
-  "simple_matcher (Dst (Ip4Addr ip)) p = bool_to_ternary (ipv4addr_of_dotteddecimal ip = dst_ip p)"
-  "simple_matcher (Dst (Ip4AddrNetmask ip n)) p = bool_to_ternary (dst_ip p \<in> ipv4range_set_from_bitmask (ipv4addr_of_dotteddecimal ip) n)"
+lemma simple_matcher_simps[simp]:
+  "simple_matcher (Src ip) p = bool_to_ternary (src_ip p \<in> ipv4s_to_set ip)"
+  "simple_matcher (Dst ip) p = bool_to_ternary (dst_ip p \<in> ipv4s_to_set ip)"
+apply(case_tac [!] ip)
 apply(auto)
 apply (metis (poly_guards_query) bool_to_ternary_simps(2))+
 done
+
+declare simple_matcher.simps(1)[simp del]
+declare simple_matcher.simps(2)[simp del]
+declare simple_matcher.simps(3)[simp del]
+declare simple_matcher.simps(4)[simp del]
+
 
 
 text{*Perform very basic optimizations*}
